---
dg-publish: true
---

On pose $\mathfrak{v}_{n}=S_{2n}$ et $\mathfrak{w}_{n}=S_{2n+1}$.
On a $\mathfrak{v}_{n+1}-\mathfrak{v_{n}}=u_{2n+2}-u_{2n+1}\leq0$
Et $\mathfrak{w}_{n+1}-\mathfrak{w}_{n}=-u_{2n+3}+u_{2n+2}\geq 0$ 
Donc $\mathfrak{v}_{n}$ est d√©croissante et $\mathfrak{w_{n}}$ croissante.
Et $\mathfrak{w_{n}}-\mathfrak{v_{n}}=(-1)^{2n+1}u_{2n+1}\xrightarrow[]{}0$
Donc $\mathfrak{w,v}$ sont adjacentes et $S_{n}$ converge.
Majorons alors $R_{n}=\sum^{+\infty}_{n} (-1)^{k}u_{k}=\left| S_{n}-\ell \right|$
On a $S_{2n+1}\leq \ell \leq S_{n}$ (petit dessin) donc
$$
\left| S_{2n}-\ell \right|\leq \left| S_{2n+1}-S_{2n} \right|= u_{2n+1}
$$
Et
$$
\left| S_{2n+1}-\ell \right|\leq \left| S_{2n+1}-S_{2n+2} \right| = u_{2n+2}
$$
