---
dg-publish: true
---

Soit $\beta$ une racine de $P'$.
- Si $\beta$ est racine de $P$, ok
- Sinon,
$$
\begin{align}
\frac{P'}{P}(\beta) &= 0 \\
\sum \frac{n_{k}}{\beta - \alpha_{k}} &= 0 \\
\sum n_{k} \frac{\overline{\beta} - \overline{\alpha}_{k}}{\left| \beta-\alpha_{k} \right|^{2}} &= 0 \\
\overline{\beta} \sum \frac{n_{k}}{\left| \beta-\alpha_{k} \right|^{2}} &= \sum \frac{n_{k}\overline{\alpha}_{k}}{\left| \beta-\alpha_{k} \right|^{2}} \\
\beta &= \frac{ \sum \frac{n_{k} \alpha _{k}}{\left| \beta-\alpha_{k} \right|^{2}} }{\sum \frac{n_{k}}{\left| \beta-\alpha _{k} \right|^{2}}}
\end{align}
$$
D'o√π le poids de $\dots$
