---
dg-publish: true
---

# $I+J$

- Soit $z\in I+J$ alors il existe $(x,y)\in I\times J$ avec $z = x + y \in A$ ok
- On a $0_{A} \in I$ et $0_{A}\in J$ donc $0_{A} \in I + J$ ok
- $z_{1},z_{2} \in I+J$ alors il existe $((x,y),(v,w))\in (I\times J)^{2}$ avec $z_{1}=x+y$ et $z_{2}=v+w$. 
Donc on a $z_{1}-z_{2}=(x+y)-(v+w)=(x-v)+(y-w) \in I+J$ ok
- $z\in I+J$ donc il existe $x,y \in I\times J$ avec $x+y=z$. Pour $t\in A$, on a $tz=tx+ty \in I+J$ ok

# $I\cap J$

- Comme $(I, +)$ et $(J,+)$ sont sous-groupes [[Preuve - Intersection sous-groupes|alors]] $(I \cap J, +)$ aussi
- Soient $z\in I \cap J$ et $t \in A$, on a $zt \in I$ et $zt \in J$ donc $zt \in I\cap J$
